ROOT
@@ -1,11 +1,14 @@
-session Tree_Enumeration = HOL +
-  options [document = pdf, document_output = "output"]
+chapter AFP
+
+session Tree_Enumeration (AFP) = HOL +
+  options [document = pdf, document_output = "output", timeout = 600]
   sessions
     "Undirected_Graph_Theory"
-    "Combinatorial_Enumeration_Algorithms"
   theories
     Tree_Graph
     Labeled_Tree_Enumeration
+    Rooted_Tree
     Rooted_Tree_Enumeration
   document_files
+    "root.bib"
     "root.tex"
